theories/Examples.v
@@ -2,7 +2,9 @@ From Coq Require Import List.
 From Coq Require Import Relations.Relation_Definitions.
 
 From Autosubst Require Import Autosubst.
-Require Import LambdaM Canonical.
+
+(* --------------- *)
+(* Auxiliary proof *)
 
 Lemma mmap_append {A: Type} (f: A -> A) (l1 l2: list A) :
   mmap f (l1 ++ l2) = (mmap f l1) ++ (mmap f l2).
@@ -10,36 +12,77 @@ Proof.
   induction l1 ; asimpl ; try rewrite IHl1 ; auto.
 Qed.
 
-Lemma step_subst :
-  (forall s t, LambdaM.step s t -> forall σ, LambdaM.step s.[σ] t.[σ])
-  /\
-  (forall l l', LambdaM.step' l l' -> forall σ, LambdaM.step' l..[σ] l'..[σ]) .
-Proof.
-  apply LambdaM.mut_comp_ind ; intros ; asimpl ;
-    try (constructor ; apply H). 
+(* --- *)
+
+Section Lambda.
+  Require Import Lambda.
   
-  - destruct b as [Beta | H].
-    + destruct Beta as [Beta1 | Beta2].
-      * induction Beta1. subst.
-        constructor. left. left. constructor. autosubst.
-      * induction Beta2. subst.
-        constructor. left. right. constructor. autosubst.
-    + induction H. subst.
-      constructor. right. constructor. auto.
-Qed.
+  Theorem nfs_are_irreducible :
+    (forall s, normal s -> ~exists t, step s t)
+    /\
+    (forall s, apps s -> ~exists t, step s t).
+  Proof.
+    apply mut_normal_ind ; intros.
+    - intro.
+      apply H.
+      destruct H0 as [t Ht].
+      inversion Ht.
+      now exists s'.
+    - intro.
+      apply H.
+      destruct H0 as [t Ht].
+      now exists t.
+    - intro.
+      now destruct H.
+    - intro.
+      destruct H1 as [t0 Ht0].
+      inversion Ht0 ; subst.
+      + inversion a.
+      + apply H. now exists s'.
+      + apply H0. now exists t'.
+  Qed.
+End Lambda.
 
-Lemma step_subst_can :
-  (forall s t, Canonical.step s t -> forall σ, Canonical.step s.[σ] t.[σ])
+Section LambdaM.
+  Require Import LambdaM.
+  
+  Lemma step_subst :
+    (forall s t, step s t -> forall σ, step s.[σ] t.[σ])
+    /\
+    (forall l l', step' l l' -> forall σ, step' l..[σ] l'..[σ]) .
+  Proof.
+    apply mut_comp_ind ; intros ; asimpl ;
+      try (constructor ; apply H). 
+    
+    - destruct b as [Beta | H].
+      + destruct Beta as [Beta1 | Beta2].
+        * induction Beta1. subst.
+          constructor. left. left. constructor. autosubst.
+        * induction Beta2. subst.
+          constructor. left. right. constructor. autosubst.
+      + induction H. subst.
+        constructor. right. constructor.
+        now rewrite mmap_append.
+  Qed.
+End LambdaM.
+
+Section Canonical.
+  Require Import Canonical.
+  
+  Lemma step_subst_can :
+  (forall s t, step s t -> forall σ, step s.[σ] t.[σ])
   /\
-  (forall l l', Canonical.step' l l' -> forall σ, Canonical.step' l..[σ] l' ..[σ]).
-Proof.
-  apply Canonical.mut_comp_ind ; intros ; autounfold ; asimpl ;
-    try (now constructor ; apply H).
+  (forall l l', step' l l' -> forall σ, step' l..[σ] l' ..[σ]).
+  Proof.
+    apply mut_comp_ind ; intros ; autounfold ; asimpl ;
+      try (now constructor ; apply H).
+    
+    - apply step_comp_app2. apply H.
+    - apply step_comp_app3. apply H.
+    - destruct b as [Beta1 | Beta2] ; constructor.
+      + induction Beta1. subst. left. constructor. autosubst.
+      + induction Beta2. subst. right. asimpl. constructor.
+        rewrite app_subst_comm. f_equal. autosubst.
+  Qed.
+End Canonical.
 
-  - apply step_comp_app2. apply H.
-  - apply step_comp_app3. apply H.
-  - destruct b as [Beta1 | Beta2] ; constructor.
-    + induction Beta1. subst. left. constructor. autosubst.
-    + induction Beta2. subst. right. asimpl. constructor.
-      rewrite app_subst_comm. f_equal. autosubst.
-Qed.
