theories/SimpleTypes.v
@@ -1,4 +1,6 @@
 (* Simple Types *)
 (* ------------ *)
 
-Inductive type: Type := Base | Arr : type -> type -> type.
+Inductive type: Type :=
+| Base
+| Arr (A B: type) : type.
