theories/TypePreservation.v
@@ -133,13 +133,14 @@ Corollary type_preservation' Γ t t' A :
   Canonical.step t t' ->
   Canonical.sequent Γ t' A.
 Proof.
+  specialize (proj1 i_is_canonical) with t'. intro it'.
+  apply h_is_surjective in it'.
+
   intros H1 H2.
   rewrite<- (proj1 inversion2) with t'.
-  apply p_is_admissible.
-  specialize (proj1 i_is_canonical) with t'. intro it'.
-  apply h_is_surjective in it'. rewrite it'. constructor.
+  apply p_is_admissible. rewrite it'. constructor.
   apply type_preservation_multistep with (t:=i t).
-  - apply i_is_admissible in H1. inversion H1.
+  - apply i_is_admissible in H1. induction H1.
     apply type_preservation_multistep with (t:=t0).
     + assumption.
     + apply multistep_H_inclusion.
